src/cbor/spec/CBOR.Spec.API.Format.fsti
@@ -210,3 +210,37 @@ val cbor_det_serialize_map_length_gt_list
     FStar.UInt.fits (cbor_map_length l) 64 /\
     Seq.length (cbor_det_serialize (pack (CMap l))) > Seq.length (cbor_det_serialize_map l)
   ))
+
+val cbor_det_parse_map
+  (n: nat)
+  (s: Seq.seq U8.t)
+: Pure (option (cbor_map & nat))
+  (requires True)
+  (ensures fun res -> match res with
+  | None -> True
+  | Some (_, len) ->
+    len <= Seq.length s
+  )
+
+val cbor_det_parse_map_prefix
+  (n: nat)
+  (s1 s2: Seq.seq U8.t)
+: Lemma
+  (match cbor_det_parse_map n s1 with
+  | None -> True
+  | Some (l, len1) ->
+    (len1 <= Seq.length s2 /\ Seq.slice s1 0 len1 == Seq.slice s2 0 len1) ==>
+    cbor_det_parse_map n s2 == Some (l, len1)
+  )
+
+val cbor_det_parse_map_equiv
+  (n: nat)
+  (s: Seq.seq U8.t)
+  (l: cbor_map)
+  (len: nat)
+: Lemma
+  (cbor_det_parse_map n s == Some (l, len) <==> (
+    n == cbor_map_length l /\
+    len <= Seq.length s /\
+    Seq.slice s 0 len == cbor_det_serialize_map l
+  ))
